`ToList` and (`Push` / `Pop`) `Front` / `Back`

Algorithm/Data/Classes/Collection.lean
@@ -5,17 +5,17 @@ Authors: Yuyang Zhao
 -/
 import Mathlib.Data.Multiset.Basic
 
-class Collection (C : Type*) (α : outParam Type*) where
-  empty : C
-  toMultiset : C → Multiset α
-  isEmpty : C → Bool
+class CollectionCore (C : Type*) (α : outParam Type*) where
   size : C → Nat
-  count : [DecidableEq α] → α → C → Nat := fun v c ↦ (toMultiset c).count v
-  count_toMultiset : [DecidableEq α] → ∀ v c,
-    (toMultiset c).count v = count v c := by intros; rfl
-  card_toMultiset_eq_size c : Multiset.card (toMultiset c) = size c
-  toMultiset_empty : toMultiset empty = 0
+  isEmpty : C → Bool
   isEmpty_iff_size_eq_zero c : isEmpty c ↔ size c = 0
+export CollectionCore (size isEmpty isEmpty_iff_size_eq_zero)
+
+-- do not need to write `toMultiset` if we have `toList`
+class Collection (C : Type*) (α : outParam Type*) extends CollectionCore C α where
+  toMultiset : C → Multiset α
+  card_toMultiset_eq_size c : Multiset.card (toMultiset c) = size c
+export Collection (toMultiset card_toMultiset_eq_size)
 
 attribute [simp] Collection.card_toMultiset_eq_size
 
@@ -23,32 +23,24 @@ section
 variable {α : Type*}
 
 instance : Collection (List α) α where
-  empty := []
   toMultiset := (↑)
   size := List.length
   card_toMultiset_eq_size c := rfl
   isEmpty := List.isEmpty
-  toMultiset_empty := rfl
   isEmpty_iff_size_eq_zero l := by cases l <;> simp
 
 instance : Collection (Array α) α where
-  empty := #[]
-  toMultiset a := ↑a.toListRev
+  toMultiset a := ↑a.toList
   size := Array.size
   card_toMultiset_eq_size c := by simp
   isEmpty := Array.isEmpty
-  toMultiset_empty := rfl
   isEmpty_iff_size_eq_zero l := by simp
 
-namespace Collection
+section Collection
 variable {C α : Type*} [Collection C α] (c : C)
 
 instance (priority := 100) : Membership α C where
   mem a c := a ∈ toMultiset c
-
-lemma isEmpty_empty : isEmpty (empty : C) := by
-  rw [isEmpty_iff_size_eq_zero, ← card_toMultiset_eq_size, toMultiset_empty]
-  rfl
 
 lemma isEmpty_eq_decide_size : isEmpty c = decide (size c = 0) := by
   simp only [← isEmpty_iff_size_eq_zero, Bool.decide_coe]
@@ -59,16 +51,20 @@ lemma isEmpty_eq_size_beq_zero : isEmpty c = (size c == 0) := by
 
 variable [DecidableEq α]
 
+def countSlow (a : α) (c : C) : Nat :=
+  (Collection.toMultiset c).count a
+
 @[simp]
-theorem count_eq_zero {a : α} {c : C} : count a c = 0 ↔ a ∉ c := by
-  rw [← count_toMultiset]
-  exact Multiset.count_eq_zero
+theorem countSlow_eq_zero {a : α} {c : C} : countSlow a c = 0 ↔ a ∉ c :=
+  Multiset.count_eq_zero
 
-theorem count_ne_zero {a : α} {c : C} : count a c ≠ 0 ↔ a ∈ c := by
-  simp [Ne.def, count_eq_zero]
+theorem countSlow_ne_zero {a : α} {c : C} : countSlow a c ≠ 0 ↔ a ∈ c := by
+  simp [Ne.def, countSlow_eq_zero]
 
-lemma mem_iff : isEmpty (empty : C) := by
-  rw [isEmpty_iff_size_eq_zero, ← card_toMultiset_eq_size, toMultiset_empty]
-  rfl
+class Count (C : Type*) (α : outParam Type*) [Collection C α] where
+  count : [DecidableEq α] → α → C → Nat
+  count_eq_countSlow : [DecidableEq α] → ∀ a c,
+    count a c = countSlow a c := by intros; rfl
+export Count (count count_eq_countSlow)
 
 end Collection
