Algorithm/Data/Classes/Container.lean
@@ -1,0 +1,39 @@
+/-
+Copyright (c) 2023 Yuyang Zhao. All rights reserved.
+Released under Apache 2.0 license as described in the file LICENSE.
+Authors: Yuyang Zhao
+-/
+import Algorithm.Data.Classes.Collection
+
+class Container (C : Type*) (α : outParam Type*) extends Collection C α where
+  empty : C
+  toMultiset_empty : toMultiset empty = 0
+export Container (toMultiset_empty)
+
+section
+variable {α : Type*}
+
+instance : Container (List α) α where
+  empty := []
+  toMultiset_empty := rfl
+
+instance : Container (Array α) α where
+  empty := #[]
+  toMultiset_empty := rfl
+
+section Container
+variable {C α : Type*} [Container C α] (c : C)
+
+instance (priority := 100) : Membership α C where
+  mem a c := a ∈ toMultiset c
+
+def mkEmpty (C) {α} [Container C α]  : C := Container.empty
+
+@[simp]
+lemma toMultiset_mkEmpty : toMultiset (mkEmpty C) = 0 := Container.toMultiset_empty
+
+lemma isEmpty_mkEmpty : isEmpty (mkEmpty C) := by
+  rw [isEmpty_iff_size_eq_zero, ← card_toMultiset_eq_size, toMultiset_mkEmpty]
+  rfl
+
+end Container
