Algorithm/Data/Classes/ToList.lean
@@ -1,0 +1,215 @@
+/-
+Copyright (c) 2023 Yuyang Zhao. All rights reserved.
+Released under Apache 2.0 license as described in the file LICENSE.
+Authors: Yuyang Zhao
+-/
+import Algorithm.Data.Classes.Collection
+
+namespace List
+variable {α : Type*} (l : List α)
+
+-- #check isEmpty_iff_eq_nil
+lemma not_isEmpty_iff_ne_nil {l : List α} : ¬l.isEmpty ↔ l ≠ [] :=
+  isEmpty_iff_eq_nil.not
+
+-- #check getLast?_isSome
+lemma head?_isSome : (head? l).isSome ↔ l ≠ [] :=
+  match l with | [] | _::_ => by simp
+
+lemma tail?_isSome : (tail? l).isSome ↔ l ≠ [] :=
+  match l with | [] | _::_ => by simp
+
+lemma head?_isSome' : (head? l).isSome = !l.isEmpty :=
+  match l with | [] | _::_ => rfl
+
+lemma tail?_isSome' : (tail? l).isSome = !l.isEmpty :=
+  match l with | [] | _::_ => rfl
+
+instance : Decidable (l = []) :=
+  match l with
+  | [] => isTrue rfl
+  | _::_ => isFalse (nomatch ·)
+
+lemma isEmpty_eq_decide_eq_nil : l.isEmpty = decide (l = []) := by
+  cases l <;> simp [isEmpty]
+
+lemma isEmpty_eq_decide_length : l.isEmpty = decide (l.length = 0) := by
+  cases l <;> simp [isEmpty]
+
+lemma isEmpty_reverse : l.reverse.isEmpty = l.isEmpty := by
+  rw [isEmpty_eq_decide_eq_nil, isEmpty_eq_decide_eq_nil]
+  simp only [reverse_eq_nil_iff]
+
+lemma reverse_dropLast (l : List α) : l.dropLast.reverse = l.reverse.tail :=
+  match l with
+  | [] | [_] => rfl
+  | x::_::_ => by
+    rw [dropLast, reverse_cons x, reverse_cons x, reverse_dropLast (_::_),
+      tail_append_of_ne_nil] <;> simp
+
+@[simp]
+lemma back?_toArray : l.toArray.back? = l.getLast? := by
+  rw [Array.back?, Array.get?_eq_data_get?, getLast?_eq_get?]
+  simp
+
+end List
+
+namespace Array
+variable {α : Type*} (a : Array α)
+
+lemma isEmpty_data {α : Type*} (a : Array α) : a.data.isEmpty = a.isEmpty := by
+  rw [List.isEmpty_eq_decide_length, isEmpty]
+
+lemma isEmpty_toList {α : Type*} (a : Array α) : a.toList.isEmpty = a.isEmpty := by
+  rw [isEmpty_data, toList_eq]
+
+lemma isEmpty_toListRev {α : Type*} (a : Array α) : a.toListRev.isEmpty = a.isEmpty := by
+  rw [toListRev_eq, List.isEmpty_reverse, isEmpty_data]
+
+@[simp]
+lemma length_data {α : Type*} (a : Array α) : a.data.length = a.size := rfl
+
+lemma length_toList {α : Type*} (a : Array α) : a.toList.length = a.size := by
+  rw [toList_eq, length_data]
+
+@[simp]
+lemma get?_data {α : Type*} (a : Array α) : a.data.get? = a.get? := by
+  ext i
+  rw [Array.get?_eq_data_get?]
+
+lemma get?_toList {α : Type*} (a : Array α) : a.toList.get? = a.get? := by
+  rw [toList_eq, get?_data]
+
+lemma get?_toListRev {α : Type*} (a : Array α) (i : Nat) (h : i < a.size) :
+    a.toListRev.get? i = a.get? (a.size - 1 - i) := by
+  rw [toListRev_eq, List.get?_reverse _ (by rwa [length_data]), get?_data]
+
+lemma head?_toListRev {α : Type*} (a : Array α) : a.toListRev.head? = a.back? := by
+  cases a.size.eq_zero_or_pos
+  case inl h =>
+    rw [toListRev_eq, back?, ← get?_data]
+    simp [List.length_eq_zero.mp h]
+  case inr h =>
+    rw [← List.get?_zero, get?_toListRev _ _ h, Nat.sub_zero]
+    rfl
+
+lemma getLast?_toList (a : Array α) : a.toList.getLast? = a.back? := by
+  rw [back?, get?_eq_data_get?, List.getLast?_eq_get?]
+  simp
+
+@[simp]
+lemma getLast?_data (a : Array α) : a.data.getLast? = a.back? := by
+  simp [← getLast?_toList]
+
+lemma dropLast_toList (a : Array α) : a.toList.dropLast = a.pop.toList := by
+  simp
+
+end Array
+
+class ToList (C : Type*) (α : outParam Type*) extends CollectionCore C α where
+  toList : C → List α
+  toArray : C → Array α
+  toArray_toList a : (toArray a).toList = toList a
+  length_toList c : (toList c).length = size c
+export ToList (toList toArray toArray_toList length_toList)
+
+section ToList
+variable {C α : Type*} [ToList C α] (c : C)
+
+instance (priority := 100) : Collection C α where
+  toMultiset c := ↑(toList c)
+  card_toMultiset_eq_size c := length_toList c
+
+lemma coe_toList_eq_toMultiset : ↑(toList c) = toMultiset c := rfl
+
+lemma isEmpty_toList : (toList c).isEmpty = isEmpty c := by
+  rw [isEmpty_eq_decide_size, List.isEmpty_eq_decide_length, length_toList]
+
+end ToList
+
+class Front (C : Type*) (α : outParam Type*) [ToList C α] where
+  front? : C → Option α
+  head?_toList s : (toList s).head? = front? s
+  frontD : C → α → α :=
+    fun s d ↦ (front? s).getD d
+  front (c : C) : ¬isEmpty c → α :=
+    fun h ↦ (front? c).get (by rwa [← head?_toList, List.head?_isSome, ← List.not_isEmpty_iff_ne_nil, isEmpty_toList])
+  frontD_def c d : frontD c d = (front? c).getD d := by intros; rfl
+  front_mem c h : front c h ∈ front? c := by simp
+export Front (front? head?_toList frontD front frontD_def front_mem)
+
+class Back (C : Type*) (α : outParam Type*) [ToList C α] where
+  back? : C → Option α
+  getLast?_toList s : (toList s).getLast? = back? s
+  backD : C → α → α :=
+    fun s d ↦ (back? s).getD d
+  back (c : C) : ¬isEmpty c → α :=
+    fun h ↦ (back? c).get (by rwa [← getLast?_toList, List.getLast?_isSome, ← List.not_isEmpty_iff_ne_nil, isEmpty_toList])
+  backD_def c d : backD c d = (back? c).getD d := by intros; rfl
+  back_mem c h : back c h ∈ back? c := by simp
+export Back (back? getLast?_toList backD back backD_def back_mem)
+
+class PopFront (C : Type*) (α : outParam Type*) [ToList C α] where
+  popFront : C → C
+  tail_toList s : (toList s).tail = toList (popFront s)
+export PopFront (popFront tail_toList)
+
+class PopBack (C : Type*) (α : outParam Type*) [ToList C α] where
+  popBack : C → C
+  dropLast_toList s : (toList s).dropLast = toList (popBack s)
+export PopBack (dropLast_toList dropLast_toList)
+
+class PushFront (C : Type*) (α : outParam Type*) [ToList C α] where
+  pushFront : C → α → C
+  cons_toList s a : List.cons a (toList s) = toList (pushFront s a)
+export PopFront (popFront tail_toList)
+
+class PushBack (C : Type*) (α : outParam Type*) [ToList C α] where
+  pushBack : C → α → C
+  toList_append_singleton s a : toList s ++ [a] = toList (pushBack s a)
+export PopFront (popFront tail_toList)
+
+section
+variable {α : Type*}
+
+instance : ToList (List α) α where
+  toList := id
+  toArray := List.toArray
+  toArray_toList _ := by simp
+  length_toList _ := rfl
+
+instance : Front (List α) α where
+  front? := List.head?
+  head?_toList _ := rfl
+  frontD := List.headD
+  front l h := l.head <| List.not_isEmpty_iff_ne_nil.mp h
+  frontD_def := List.headD_eq_head?
+  front_mem _ _ := List.head?_eq_head _ _
+
+instance : PopFront (List α) α where
+  popFront := List.tail
+  tail_toList _ := rfl
+
+instance : PushFront (List α) α where
+  pushFront c a := List.cons a c
+  cons_toList _ _ := rfl
+
+instance : ToList (Array α) α where
+  toList := Array.toList
+  toArray := id
+  toArray_toList _ := rfl
+  length_toList _ := by simp [size]
+
+instance : Back (Array α) α where
+  back? := Array.back?
+  getLast?_toList := Array.getLast?_toList
+
+instance : PopBack (Array α) α where
+  popBack := Array.pop
+  dropLast_toList := Array.dropLast_toList
+
+instance : PushBack (Array α) α where
+  pushBack := Array.push
+  toList_append_singleton _ _ := by simp [toList]
+
+end
